feat: EquivManager finished 🎉

Lean4Lean/Theory/VExpr.lean
@@ -510,15 +510,24 @@ inductive Lift : Type where
   | skip : Lift → Lift
   | cons : Lift → Lift
 
-@[simp] def Lift.skipN : Nat → Lift
-  | 0   => .refl
-  | n+1 => .skip (Lift.skipN n)
+namespace Lift
 
-@[simp] def Lift.consN (l : Lift) : Nat → Lift
+@[simp] def skipN (l : Lift) : Nat → Lift
+  | 0   => l
+  | n+1 => .skip (skipN l n)
+
+theorem skipN_one : skipN l 1 = .skip l := rfl
+
+theorem skipN_skipN : skipN (skipN l n) k = skipN l (n + k) := by induction k <;> simp [*]
+
+@[simp] def consN (l : Lift) : Nat → Lift
   | 0  => l
-  | k+1 => .cons (Lift.consN l k)
+  | k+1 => .cons (consN l k)
 
-@[simp] def Lift.comp (l₁ l₂ : Lift) : Lift :=
+theorem consN_consN : consN (.consN l a) b = .consN l (a + b) := by
+  induction b <;> simp [*]
+
+@[simp] def comp (l₁ l₂ : Lift) : Lift :=
   match l₂, l₁ with
   | .refl,    l₁       => l₁
   | .skip l₂, l₁       => .skip (l₁.comp l₂)
@@ -526,68 +535,76 @@ inductive Lift : Type where
   | .cons l₂, .skip l₁ => .skip (l₁.comp l₂)
   | .cons l₂, .cons l₁ => .cons (l₁.comp l₂)
 
-@[simp] def Lift.depth : Lift → Nat
+@[simp] theorem refl_comp : comp refl l = l := by induction l <;> simp [*]
+
+theorem consN_comp : consN (.comp l₁ l₂) n = .comp (.consN l₁ n) (.consN l₂ n) := by
+  induction n <;> simp [*]
+
+@[simp] def depth : Lift → Nat
   | .refl   => 0
   | .skip l => l.depth + 1
   | .cons l => l.depth
 
-theorem Lift.depth_comp : Lift.depth (.comp l₁ l₂) = l₁.depth + l₂.depth :=
+theorem depth_comp : depth (.comp l₁ l₂) = l₁.depth + l₂.depth :=
   match l₂, l₁ with
   | .refl,    _        => rfl
-  | .skip _,  _        => congrArg Nat.succ Lift.depth_comp
+  | .skip _,  _        => congrArg Nat.succ depth_comp
   | .cons _,  .refl    => (Nat.zero_add _).symm
-  | .cons _,  .skip _  => (congrArg Nat.succ Lift.depth_comp).trans (Nat.succ_add ..).symm
-  | .cons l₂, .cons l₁ => @Lift.depth_comp l₁ l₂
+  | .cons _,  .skip _  => (congrArg Nat.succ depth_comp).trans (Nat.succ_add ..).symm
+  | .cons l₂, .cons l₁ => @depth_comp l₁ l₂
 
-@[simp] theorem Lift.depth_consN : Lift.depth (.consN l n) = l.depth := by induction n <;> simp [*]
+@[simp] theorem depth_consN : depth (.consN l n) = l.depth := by induction n <;> simp [*]
 
-theorem Lift.consN_consN : Lift.consN (.consN l a) b = .consN l (a + b) := by
-  induction b <;> simp [*]
+@[simp] theorem depth_skipN : depth (.skipN l n) = l.depth + n := by
+  induction n <;> simp [Nat.add_assoc, *]
 
-theorem Lift.consN_comp : Lift.consN (.comp l₁ l₂) n = .comp (.consN l₁ n) (.consN l₂ n) := by
-  induction n <;> simp [*]
-
-@[simp] theorem Lift.depth_skipN : Lift.depth (.skipN n) = n := by induction n <;> simp [*]
-
-theorem Lift.consN_skip_eq : consN (skip l) k = comp (consN l k) (consN (skipN 1) k) := by
+theorem consN_skip_eq : consN (skip l) k = comp (consN l k) (consN (skip refl) k) := by
   rw [← consN_comp]; rfl
 
-theorem Lift.depth_succ (H : l.depth = n + 1) :
-    ∃ l' k, Lift.depth l' = n ∧ l = Lift.consN (.skip l') k := by
+theorem depth_succ (H : l.depth = n + 1) :
+    ∃ l' k, depth l' = n ∧ l = consN (.skip l') k := by
   match l with
   | .skip l => cases H; exact ⟨l, 0, rfl, rfl⟩
   | .cons l =>
     obtain ⟨l, k, rfl, ⟨⟩⟩ := depth_succ (l := l) H
     exact ⟨l, k+1, rfl, rfl⟩
 
-theorem Lift.depth_succ' (H : l.depth = n + 1) :
-    ∃ l' k, Lift.depth l' = n ∧ l = Lift.comp l' (.consN (.skipN 1) k) := by
+theorem depth_succ' (H : l.depth = n + 1) :
+    ∃ l' k, depth l' = n ∧ l = comp l' (.consN (.skip refl) k) := by
   let ⟨l', k, h1, h2⟩ := depth_succ H
   exact ⟨.consN l' k, k, by simp [h1], by rwa [← consN_skip_eq]⟩
 
-@[simp] def Lift.liftVar : Lift → Nat → Nat
+theorem comp_skipN : comp l₁ (skipN l₂ k) = skipN (comp l₁ l₂) k := by
+  induction k <;> simp [*]
+
+theorem skipN_comp_consN : comp (skipN l₁ k) (consN l₂ k) = skipN (comp l₁ l₂) k := by
+  induction k <;> simp [*]
+
+@[simp] protected def liftVar : Lift → Nat → Nat
   | .refl, n => n
   | .skip l, n => l.liftVar n + 1
   | .cons _, 0 => 0
   | .cons l, n+1 => l.liftVar n + 1
 
-theorem liftVar_comp : Lift.liftVar (.comp l₁ l₂) n = l₂.liftVar (l₁.liftVar n) := by
+theorem liftVar_comp : (comp l₁ l₂).liftVar n = l₂.liftVar (l₁.liftVar n) := by
   induction l₂ generalizing l₁ n <;> [skip; skip; cases l₁ <;> [skip; skip; cases n]] <;> simp [*]
 
-theorem liftVar_skipN : (Lift.skipN n).liftVar i = i + n := by
+theorem liftVar_skipN : (skipN l n).liftVar i = l.liftVar i + n := by
   induction n generalizing i with
   | zero => rfl
   | succ _ ih => simp [ih]; rfl
 
-theorem liftVar_consN_skipN : (Lift.consN (.skipN n) k).liftVar i = liftVar n i k := by
+theorem liftVar_consN_skipN : (consN (skipN refl n) k).liftVar i = liftVar n i k := by
   induction k generalizing i with
   | zero => simp [liftVar_skipN]
   | succ k ih =>
     cases i with simp [liftVar, Nat.succ_lt_succ_iff, ih]
     | succ i => split <;> rfl
 
-theorem liftVar_depth_zero (H : l.depth = 0) : Lift.liftVar l n = n := by
-  induction l generalizing n <;> [skip; skip; cases n] <;> simp_all [Lift.depth]
+theorem liftVar_depth_zero (H : depth l = 0) : l.liftVar n = n := by
+  induction l generalizing n <;> [skip; skip; cases n] <;> simp_all [depth]
+
+end Lift
 
 namespace VExpr
 
@@ -599,11 +616,13 @@ namespace VExpr
   | .lam ty body, k => .lam (ty.lift' k) (body.lift' k.cons)
   | .forallE ty body, k => .forallE (ty.lift' k) (body.lift' k.cons)
 
-theorem lift'_consN_skipN : e.lift' (.consN (.skipN n) k) = liftN n e k := Eq.symm <| by
-  induction e generalizing k <;> simp [liftN, liftVar_consN_skipN, *]
+theorem lift'_consN_skipN : e.lift' (.consN (.skipN .refl n) k) = liftN n e k := Eq.symm <| by
+  induction e generalizing k <;> simp [liftN, Lift.liftVar_consN_skipN, *]
 
 theorem lift'_comp {e : VExpr} : e.lift' (.comp l₁ l₂) = (e.lift' l₁).lift' l₂ := Eq.symm <| by
-  induction e generalizing l₁ l₂ <;> simp [liftVar_comp, *]
+  induction e generalizing l₁ l₂ <;> simp [Lift.liftVar_comp, *]
 
 theorem lift'_depth_zero {e : VExpr} (H : l.depth = 0) : e.lift' l = e := by
-  induction e generalizing l <;> simp_all [liftVar_depth_zero]
+  induction e generalizing l <;> simp_all [Lift.liftVar_depth_zero]
+
+@[simp] theorem lift'_refl {e : VExpr} : e.lift' .refl = e := lift'_depth_zero rfl
