Lean4Lean/Std/Basic.lean
@@ -1,6 +1,7 @@
 import Batteries.CodeAction
 import Batteries.Data.Array.Lemmas
 import Batteries.Data.HashMap.Basic
+import Batteries.Data.UnionFind.Basic
 import Batteries.Tactic.SeqFocus
 
 open Std
@@ -194,3 +195,26 @@ instance : LawfulEqOrd UInt64 where
   eq_of_compare := compareOfLessAndEq_eq_eq UInt64.le_refl UInt64.not_le |>.mp
 
 end UInt64
+
+namespace Batteries.UnionFind
+
+@[simp] theorem size_push (uf : UnionFind) : uf.push.size = uf.size + 1 := by
+  simp [push, size]
+
+@[simp] theorem size_link (uf : UnionFind) (i j hi) : (uf.link i j hi).size = uf.size := by
+  simp [link, size]
+
+@[simp] theorem size_union (uf : UnionFind) (i j) : (uf.union i j).size = uf.size := by
+  simp [union, size]
+
+theorem Equiv.eq_of_ge_size (h : Equiv uf a b) (h2 : uf.size ≤ a) : a = b := by
+  simp [Equiv, rootD, Nat.not_lt.2 h2] at h; split at h
+  · have := (uf.root ⟨b, ‹_›⟩).2; omega
+  · exact h
+
+theorem Equiv.lt_size (h : Equiv uf a b) : a < uf.size ↔ b < uf.size :=
+  suffices ∀ {a b}, Equiv uf a b → b < uf.size → a < uf.size from ⟨this h.symm, this h⟩
+  fun h h1 => Nat.not_le.1 fun h2 => Nat.not_le.2 h1 <| h.eq_of_ge_size h2 ▸ h2
+
+
+end Batteries.UnionFind
